Rules.thy
@@ -22,7 +22,7 @@ inductive rules :: "'b rpred \<Rightarrow> 'b rpred \<Rightarrow> 'b set \<Right
   seq[intro]:    "R,G \<turnstile> Q { c\<^sub>2 } M \<Longrightarrow> R,G \<turnstile> P { c\<^sub>1 } Q \<Longrightarrow> R,G \<turnstile> P { c\<^sub>1 ;; c\<^sub>2 } M" |
   choice[intro]: "R,G \<turnstile> P { c\<^sub>1 } Q \<Longrightarrow> R,G \<turnstile> P { c\<^sub>2 } Q \<Longrightarrow> R,G \<turnstile> P { c\<^sub>1 \<sqinter> c\<^sub>2 } Q" |
   loop[intro]:   "stable R P \<Longrightarrow> R,G \<turnstile> P { c } P \<Longrightarrow> R,G \<turnstile> P { c* } P" |
-  thread[intro]: "R,G \<turnstile> P { c } Q \<Longrightarrow> inter R G c \<Longrightarrow> R,G \<turnstile> P { Thread c } Q" |
+  thread[intro]: "R,G \<turnstile> P { c } Q \<Longrightarrow> rif R G c \<Longrightarrow> R,G \<turnstile> P { Thread c } Q" |
   par[intro]:    "R\<^sub>1,G\<^sub>1 \<turnstile> P\<^sub>1 { c\<^sub>1 } Q\<^sub>1 \<Longrightarrow> R\<^sub>2,G\<^sub>2 \<turnstile> P\<^sub>2 { c\<^sub>2 } Q\<^sub>2 \<Longrightarrow> G\<^sub>2 \<subseteq> R\<^sub>1 \<Longrightarrow> G\<^sub>1 \<subseteq> R\<^sub>2 \<Longrightarrow> 
                   R\<^sub>1 \<inter> R\<^sub>2,G\<^sub>1 \<union> G\<^sub>2 \<turnstile> P\<^sub>1 \<inter> P\<^sub>2 { c\<^sub>1 || c\<^sub>2 } (Q\<^sub>1 \<inter> Q\<^sub>2)" |
   conseq[intro]: "R,G \<turnstile> P { c } Q \<Longrightarrow> P' \<subseteq> P \<Longrightarrow> R' \<subseteq> R \<Longrightarrow> G \<subseteq> G' \<Longrightarrow> Q \<subseteq> Q' \<Longrightarrow> 
