SimAsm/SimAsm_Inter.thy
@@ -1,0 +1,528 @@
+theory SimAsm_Inter
+  imports SimAsm_WP "HOL-Library.While_Combinator"
+begin
+
+record ('v,'g,'r,'a) point =
+  op  :: "('v,'g,'r,'a) opbasic"
+  rgs :: "'r set"          
+  wrs :: "'g set"
+  rds :: "'g set"
+  fen :: bool
+  inv :: bool
+
+fun upd_assign
+  where 
+    "upd_assign (Reg r) e p = p" |
+    "upd_assign (Glb g) e p = p"
+
+fun upd_cmp
+  where
+    "upd_cmp b p = p"
+
+abbreviation shr
+  where "shr A \<equiv> {g. Glb g \<in> A}"
+
+abbreviation priv
+  where "priv A \<equiv> {g. Reg g \<in> A}"
+
+abbreviation inst
+  where "inst a \<equiv> fst (tag a)"
+
+fun ord
+  where
+    "ord nop p = False" |
+    "ord (cmp b) p = (wrs p \<noteq> {} \<or> shr (deps\<^sub>B b) \<inter> rds p \<noteq> {})" |
+    "ord (assign (Reg r) e) p = (shr (deps e) \<inter> (rds p \<union> wrs p) \<noteq> {} \<or> (r \<in> rgs p \<and> shr (deps e) \<noteq> {}))" |
+    "ord (assign (Glb x) e) p = (shr (deps e) \<inter> (rds p \<union> wrs p) \<noteq> {} \<or> x \<in> wrs p)" |
+    "ord full_fence _ = True"
+
+fun wp\<^sub>b :: "('v,'g,'a) grel \<Rightarrow> ('v,'g,'r,'a) opbasic \<Rightarrow> ('v,'g,'r,'a) trans"
+  where "wp\<^sub>b R ((\<alpha>,f),v,_) Q = stabilize R (v \<inter> wp\<^sub>i \<alpha> (wp\<^sub>a f Q))"
+
+fun chk :: "('v,'g,'a) grel \<Rightarrow> ('v,'g,'r,'a) opbasic \<Rightarrow> ('v,'g,'r,'a) point \<Rightarrow> bool"
+  where
+    "chk R a p = 
+      (inst a = full_fence \<or>
+      (\<forall>Q. stable\<^sub>t R Q \<longrightarrow> wp\<^sub>b Id a (wp\<^sub>b R (op p) Q) \<subseteq> wp\<^sub>b Id (op p) (wp\<^sub>b R a Q)))"
+
+fun stren :: "('v,'g,'r) op \<Rightarrow> ('v,'g,'r,'a) point \<Rightarrow> ('v,'g,'r,'a) point"
+  where
+    "stren a p = p\<lparr> rgs := rgs p - priv (wr a) \<union> priv (rd a), 
+                    wrs := wrs p \<union> shr (wr a), 
+                    rds := rds p \<union> shr (rd a), 
+                    fen := fen p \<or> (a = full_fence) \<rparr>"
+
+fun weaken :: "('v,'g,'r) op \<Rightarrow> ('v,'g,'r,'a) point \<Rightarrow> ('v,'g,'r,'a) point"
+  where
+    "weaken a p = p\<lparr> rds := rds p - shr (wr a) \<rparr>"
+
+fun upd\<^sub>i
+  where
+    "upd\<^sub>i R a p = (if fen p \<or> ord (inst a) p then stren (inst a) p 
+                  else (weaken (inst a) p)\<lparr>inv := inv p \<and> chk R a p\<rparr>)"
+
+definition gen
+  where
+    "gen a = \<lparr> op = a, 
+              rgs = priv (rd (inst a)), 
+              wrs = shr (wr (inst a)), 
+              rds = shr (rd (inst a)), 
+              fen = (inst a = full_fence),
+              inv = True\<rparr>"
+
+definition upd\<^sub>a
+  where "upd\<^sub>a R a P = ({ gen a } \<union> ((upd\<^sub>i R a) ` P))"
+
+fun upd2
+  where 
+    "upd2 R (Basic a) P = upd\<^sub>a R a P" |
+    "upd2 R (Choice c\<^sub>1 c\<^sub>2) P = (upd2 R c\<^sub>1 P \<union> upd2 R c\<^sub>2 P)" |
+    "upd2 R (Loop c) P = lfp (\<lambda>Y. (P \<union> upd2 R c Y))" |
+    "upd2 R (c\<^sub>1 ;; c\<^sub>2) P = upd2 R c\<^sub>1 (upd2 R c\<^sub>2 P)" |
+    "upd2 R _ P = P"
+
+declare upd2.simps(3)[simp del]
+
+lemma mono_upd\<^sub>a:
+  "mono (upd\<^sub>a R a)"
+  by (smt Un_mono image_Un monoI order_refl sup.orderE sup_ge2 upd\<^sub>a_def)
+
+lemma mono_upd:
+  "mono (upd2 R c)"
+proof (induct c)
+  case (Seq c1 c2)
+  then show ?case by (simp add: mono_def)
+next
+  case (Choice c1 c2)
+  then show ?case
+    by (smt Un_mono mono_def upd2.simps(2))
+next
+  case (Loop c)
+  then show ?case 
+    by (smt Un_iff lfp_mono monoI subset_eq upd2.simps(3))
+qed (simp add: monoI mono_upd\<^sub>a)+
+
+lemma mono_union_upd2:
+  "mono (\<lambda>Y. (P \<union> upd2 R c Y))"
+  by (smt Un_mono monoD monoI mono_upd sup.idem sup.order_iff)
+
+subsection \<open>Correctness\<close>
+
+lemma upd_rw:
+  assumes "c \<leadsto> c'" "local c"
+  shows "upd2 R c' P \<subseteq> upd2 R c P"
+  using assms
+proof (induct arbitrary: P)
+  case (seq2 c\<^sub>2 c\<^sub>2' c\<^sub>1)
+  then show ?case by (simp add: monoD mono_upd)
+next
+  case (loop1 c)
+  then show ?case unfolding upd2.simps
+    using def_lfp_unfold[OF _ mono_union_upd2] by blast
+next
+  case (loop2 c)
+  then show ?case unfolding upd2.simps
+    using def_lfp_unfold[OF _ mono_union_upd2] by blast
+qed auto
+
+lemma upd_exec:
+  assumes "lexecute c r \<alpha> c'"
+  assumes "\<forall>p \<in> upd2 R c P. inv p"
+  shows "inter\<^sub>c (step\<^sub>t R) (step G) r \<alpha> \<and> (\<forall>p \<in> upd2 R c' P. inv p)"
+  sorry
+
+lemma upd\<^sub>aI1:
+  assumes "p \<in> P"
+  shows "ord (inst \<alpha>) p \<longrightarrow> stren (inst \<alpha>) p \<in> upd\<^sub>a R \<alpha> P"
+        "\<not> ord (inst \<alpha>) p \<longrightarrow> (weaken (inst \<alpha>) p)\<lparr>inv := inv p \<and> chk R \<alpha> p\<rparr> \<in> upd\<^sub>a R \<alpha> P"
+  using assms unfolding upd\<^sub>a_def by auto
+
+lemma inv_orig\<^sub>a [intro]:
+  assumes "\<forall>x\<in>upd\<^sub>a R \<alpha> P. point.inv x" shows "\<forall>p \<in> P. inv p"
+proof (clarsimp)
+    fix x assume a: "x \<in> P"
+    show "point.inv x" 
+    proof (cases "ord (inst \<alpha>) x")
+      case True
+      hence "stren (inst \<alpha>) x \<in> upd\<^sub>a R \<alpha> P" using upd\<^sub>aI1[OF a, of \<alpha>] by simp
+      then show ?thesis using assms by auto
+    next
+      case False
+      hence "(weaken (inst \<alpha>) x)\<lparr>inv := inv x \<and> chk R \<alpha> x\<rparr> \<in> upd\<^sub>a R \<alpha> P"
+        using upd\<^sub>aI1[OF a, of \<alpha>] by simp
+      then show ?thesis using assms by auto
+    qed
+  qed
+
+lemma inv_orig [intro]:
+  assumes "\<forall>p \<in> upd2 R c P. inv p"
+  shows "\<forall>p \<in> P. inv p"
+  using assms
+proof (induct c arbitrary: P)
+  case (Basic x)
+  then show ?case using inv_orig\<^sub>a by fastforce
+next
+  case (Seq c1 c2)
+  then show ?case unfolding upd2.simps by blast
+next
+  case (Choice c1 c2)
+  then show ?case unfolding upd2.simps by blast
+next
+  case (Loop c)
+  then show ?case unfolding upd2.simps 
+    using lfp_unfold mono_union_upd2 by blast 
+qed (unfold upd2.simps, blast)
+
+definition point_cmp
+  where "point_cmp a b \<equiv> rgs a \<subseteq> rgs b \<and> wrs a \<subseteq> wrs b \<and> rds a \<subseteq> rds b"
+
+lemma point_cmp_refl [intro]:
+  "point_cmp a a"
+  by (auto simp: point_cmp_def)
+
+lemma [simp]:
+  "deps (subst e r e') = deps e - {r} \<union> (if r \<in> deps e then deps e' else {})"
+  sorry
+
+lemma [simp]:
+  "deps\<^sub>B (subst\<^sub>B e r e') = deps\<^sub>B e - {r} \<union> (if r \<in> deps\<^sub>B e then deps e' else {})"
+  sorry
+
+
+lemma upd_reorder_com:
+  assumes "reorder_com \<alpha>' c \<alpha>" "p \<in> P" "point_cmp p (gen \<alpha>)" 
+  shows "\<exists>p'. p' \<in> upd2 R c P \<and> op p' = op p \<and> point_cmp p' (gen \<alpha>')"
+  using assms
+  sorry (*
+proof (induct rule: reorder_com.induct)
+  case (2 \<alpha>' \<beta> \<alpha>)
+  hence [simp]: "op p = \<alpha>'" by auto
+  have "\<not> ord (inst \<beta>) p"
+    using 2(1,4)
+    apply (cases "inst \<beta>"; cases "tag \<beta>"; cases "\<alpha>'")
+    apply (auto simp: gen_def point_cmp_def)
+    prefer 3
+    apply (subgoal_tac "Glb x \<in> rd aa"; blast)
+    prefer 2
+    apply (subgoal_tac "Glb x \<in> wr aa"; blast)
+    apply (case_tac x11, simp)
+    apply (case_tac aa, simp split: if_splits)
+
+    apply (elim impE)
+    apply (subgoal_tac "rds p \<subseteq> shr ((deps x12a - {Reg x1} \<union> deps x12))")
+    apply (subgoal_tac "shr (insert (Reg x1) (deps x12)) \<inter> shr (deps x12a - {Reg x1} \<union> deps x12) = {}")
+    apply blast
+    apply blast
+    apply auto[1]
+
+    apply (elim conjE exE)
+    apply (subgoal_tac "Glb x \<in> insert (Reg x1) (deps x12)")
+    apply (subgoal_tac "Glb x \<in> (deps x12a - {Reg x1} \<union> deps x12)")
+    apply auto[3]
+
+    apply (elim impE)
+    apply (subgoal_tac "rds p \<subseteq> shr ((deps x12a ))")
+    apply (subgoal_tac "shr ( (deps x12)) \<inter> shr (deps x12a ) = {}")
+    apply blast
+    apply blast
+    apply blast
+
+    apply (elim conjE exE)
+    apply (subgoal_tac "Glb x \<in> insert (Reg x1) (deps x12)")
+    apply (subgoal_tac "Glb x \<in> (deps x12a - {Reg x1} \<union> deps x12)")
+    apply auto[3]
+
+    apply (simp split: if_splits)
+    apply (elim impE)
+
+    apply (subgoal_tac "rds p \<subseteq> shr (deps\<^sub>B x2 - {Reg x1} \<union> deps x12)")
+    apply (subgoal_tac "shr (insert (Reg x1) (deps x12)) \<inter> shr (deps\<^sub>B x2 - {Reg x1} \<union> deps x12) = {}")
+    apply blast
+    apply blast
+    apply auto[1]
+
+    apply (elim conjE exE)
+    apply (subgoal_tac "Glb x \<in> insert (Reg x1) (deps x12)")
+    apply (subgoal_tac "Glb x \<in> (deps\<^sub>B x2 - {Reg x1} \<union> deps x12)")
+    apply auto[3]
+
+    apply (subgoal_tac "rds p \<subseteq> shr (deps\<^sub>B x2 )")
+    apply (subgoal_tac "shr (insert (Reg x1) (deps x12)) \<inter> shr (deps\<^sub>B x2 ) = {}")
+    apply blast
+    apply blast
+    apply auto[1]
+
+    apply simp
+    apply simp
+
+    apply simp
+
+    apply (case_tac aa, simp split: if_splits)
+    apply blast
+    apply blast
+
+    apply (simp split: if_splits)
+    apply blast
+    apply blast
+
+    apply (simp split: if_splits)
+    apply (simp split: if_splits)
+    done
+
+  hence "(weaken (inst \<beta>) p)\<lparr>inv := inv p \<and> chk R \<beta> p\<rparr> \<in> upd\<^sub>a R \<beta> P"
+    using 2 by (auto simp: upd\<^sub>a_def)
+
+  moreover have "point_cmp ((weaken (inst \<beta>) p)\<lparr>inv := inv p \<and> chk R \<beta> p\<rparr>) (gen \<alpha>)"
+    using 2(1,4) unfolding point_cmp_def gen_def
+    apply auto
+    apply (cases \<alpha>'; cases \<beta>; case_tac a; case_tac aa; case_tac ab; case_tac ac; simp split: if_splits)
+    
+    sorry
+
+  moreover have "op ((weaken (inst \<beta>) p)\<lparr>inv := inv p \<and> chk R \<beta> p\<rparr>) = \<alpha>'" using 2 by auto
+
+  ultimately show ?case by auto
+next
+  case (3 \<alpha>' c\<^sub>1 c\<^sub>2 \<alpha>)
+  then show ?case
+    apply simp
+    sorry
+qed auto
+*)
+
+lemma execute_act:
+  assumes "lexecute c r \<alpha> c'"
+  shows "\<exists>p. p \<in> upd2 R c P \<and> op p = \<alpha> \<and> point_cmp p (gen (fwd_com \<alpha> r))"
+  using assms
+proof (induct arbitrary: P)
+  case (act \<alpha>)
+  have "gen \<alpha> \<in> upd\<^sub>a R \<alpha> P" by (auto simp: upd\<^sub>a_def)
+  then show ?case by (auto simp: gen_def)
+next
+  case (ino c\<^sub>1 r \<alpha> c\<^sub>1' c\<^sub>2)
+  then show ?case by simp
+next
+  case (ooo c\<^sub>1 r \<alpha> c\<^sub>1' \<alpha>' c\<^sub>2)
+  obtain p where p: "p \<in> upd2 R c\<^sub>1 P" "op p = \<alpha>" "point_cmp p (gen (fwd_com \<alpha> r))"
+    using ooo by blast
+  have r: "reorder_com \<alpha>' (c\<^sub>2) (fwd_com \<alpha> r)" using ooo by auto
+  then show ?case using p(2) upd_reorder_com[OF r p(1,3), of R] by auto
+qed
+
+lemma upd_po:
+  assumes "reorder_com \<alpha>' c \<alpha>" "p \<in> P" "point_cmp p (gen \<alpha>)" "\<alpha> = fwd_com (op p) r" "\<forall>a\<in>upd2 R c P. point.inv a"
+  shows "inter\<^sub>c (step\<^sub>t R) (step G) c \<alpha>"
+  using assms
+proof (induct \<alpha>' c \<alpha> arbitrary: P rule: reorder_com.induct)
+  case (2 \<alpha>' \<beta> \<alpha>)
+  hence "\<not> ord (inst \<beta>) p" sorry (* correctness of ordering analysis *)
+  hence "(weaken (inst \<beta>) p)\<lparr>inv := inv p \<and> chk R \<beta> p\<rparr> \<in> upd\<^sub>a R \<beta> P"
+    using 2(2) unfolding upd\<^sub>a_def upd2.simps upd\<^sub>i.simps by auto
+  hence "chk R \<beta> p" using 2 by auto
+  then show ?case
+    apply simp
+    sorry (* correctness of chk *)
+next
+  case (3 \<alpha>' c\<^sub>1 c\<^sub>2 \<alpha>)
+  then show ?case sorry
+qed auto
+
+lemma upd_exec':
+  assumes "lexecute c r \<alpha> c'"
+  assumes "\<forall>p \<in> upd2 R c P. inv p"
+  shows "inter\<^sub>c (step\<^sub>t R) (step G) r \<alpha>"
+  using assms
+proof (induct arbitrary: P)
+  case (act \<alpha>)
+  then show ?case by auto
+next
+  case (ino c\<^sub>1 r \<alpha> c\<^sub>1' c\<^sub>2)
+  then show ?case by auto
+next
+  case (ooo c\<^sub>1 r \<alpha> c\<^sub>1' \<alpha>' c\<^sub>2)
+  then obtain p where p: "p \<in> upd2 R c\<^sub>1 P" "op p = \<alpha>" "point_cmp p (gen (fwd_com \<alpha> r))"
+    using execute_act by blast
+  have r: "reorder_com \<alpha>' (c\<^sub>2) (fwd_com \<alpha> r)" using ooo by auto
+  have f: "fwd_com \<alpha> r = fwd_com (op p) r" using p by auto
+  have "inter\<^sub>c (step\<^sub>t R) (step G) r \<alpha>" using ooo inv_orig by force
+  thus ?case using upd_po[OF r p(1,3) f] ooo(4) by auto
+qed
+
+lemma upd\<^sub>aE:
+  assumes "x \<in> upd\<^sub>a R \<alpha> P"
+  obtains (ord) p where "ord (inst \<alpha>) p" "x = stren (inst \<alpha>) p" "p \<in> P" |
+          (ooo) p where "\<not> ord (inst \<alpha>) p" "x = (weaken (inst \<alpha>) p)\<lparr>inv := inv p \<and> chk R \<alpha> p\<rparr>" "p \<in> P" |
+          (gen) "x = gen \<alpha>"
+proof -
+  have "x = gen \<alpha> \<or> x \<in> upd\<^sub>i R \<alpha> ` P" using assms by (auto simp: upd\<^sub>a_def)
+  thus ?thesis
+  proof (elim disjE)
+    assume "x = gen \<alpha>"
+    thus ?thesis using gen by auto
+  next
+    assume "x \<in> upd\<^sub>i R \<alpha> ` P"
+    then obtain p where p: "p \<in> P" "x = upd\<^sub>i R \<alpha> p" by blast
+    thus ?thesis
+    proof (cases "ord (inst \<alpha>) p")
+      case True
+      thus ?thesis using p ord by auto
+    next
+      case False
+      thus ?thesis using p ooo by auto
+    qed
+  qed
+qed
+
+lemma upd_exec'':
+  assumes "lexecute c r \<alpha> c'"
+  assumes "\<forall>p \<in> upd2 R c P. inv p"
+  shows "\<forall>p \<in> upd2 R c' P. inv p"
+  using assms
+proof (induct arbitrary: P)
+  case (act \<alpha>)
+  then show ?case
+  proof (clarsimp)
+    fix x assume a: "x \<in> P"
+    show "point.inv x" 
+    proof (cases "ord (inst \<alpha>) x")
+      case True
+      hence "stren (inst \<alpha>) x \<in> upd\<^sub>a R \<alpha> P" using upd\<^sub>aI1[OF a, of \<alpha>] by simp
+      then show ?thesis using act by auto
+    next
+      case False
+      hence "(weaken (inst \<alpha>) x)\<lparr>inv := inv x \<and> chk R \<alpha> x\<rparr> \<in> upd\<^sub>a R \<alpha> P"
+        using upd\<^sub>aI1[OF a, of \<alpha>] by simp
+      then show ?thesis using act by auto
+    qed
+  qed
+next
+  case (ino c\<^sub>1 r \<alpha> c\<^sub>1' c\<^sub>2)
+  then show ?case by auto
+next
+  case (ooo c\<^sub>1 r \<alpha> c\<^sub>1' \<alpha>' c\<^sub>2)
+  then show ?case apply auto sorry
+qed
+
+theorem try_again:
+  assumes "reorder_trace t c" "local c"
+  assumes "\<forall>p \<in> upd2 R c P. inv p"
+  shows "\<forall>(r,\<alpha>) \<in> set t. inter\<^sub>c (step\<^sub>t R) (step G) r \<alpha>"
+  using assms
+proof (induct)
+  case (1 c)
+  then show ?case by auto
+next
+  case (2 c c' t)
+  then show ?case using upd_rw[OF 2(1)] local_silent by blast
+next
+  case (3 c r \<alpha> c' t)
+  then show ?case using upd_exec[OF 3(1,5), of G] local_execute[OF 3(1,4)] by auto
+qed
+
+theorem upd_correct:
+  assumes "\<forall>p \<in> upd2 R (lift\<^sub>c c) P. inv p"
+  shows "rif (step\<^sub>t R) (step G) (lift\<^sub>c c)"
+  using assms unfolding rif_def
+proof (intro impI allI ballI, goal_cases)
+  case (1 t x)
+  have l: "local (lift\<^sub>c c)" by blast
+  then show ?case using try_again[OF 1(2) l 1(1)] 1(3) by auto
+qed
+
+fun com_rgs
+  where 
+    "com_rgs (Basic a) = priv (rd (fst (tag a)))" |
+    "com_rgs (com.Seq c\<^sub>1 c\<^sub>2) = com_rgs c\<^sub>1 \<union> com_rgs c\<^sub>2" |
+    "com_rgs (Choice c\<^sub>1 c\<^sub>2) = com_rgs c\<^sub>1 \<union> com_rgs c\<^sub>2" |
+    "com_rgs (Loop c) = com_rgs c" |
+    "com_rgs _ = {}"
+
+fun com_glbs
+  where 
+    "com_glbs (Basic a) = shr (rd (fst (tag a))) \<union> shr (wr (fst (tag a)))" |
+    "com_glbs (com.Seq c\<^sub>1 c\<^sub>2) = com_glbs c\<^sub>1 \<union> com_glbs c\<^sub>2" |
+    "com_glbs (Choice c\<^sub>1 c\<^sub>2) = com_glbs c\<^sub>1 \<union> com_glbs c\<^sub>2" |
+    "com_glbs (Loop c) = com_glbs c" |
+    "com_glbs _ = {}"
+
+
+(*
+
+fun prog_rgs
+  where 
+    "prog_rgs Skip = {}" |
+    "prog_rgs (Op v e f) = priv (rd e)" |
+    "prog_rgs (Seq c\<^sub>1 c\<^sub>2) = prog_rgs c\<^sub>1 \<union> prog_rgs c\<^sub>2" |
+    "prog_rgs (If b c\<^sub>1 c\<^sub>2) = priv (deps\<^sub>B b) \<union> prog_rgs c\<^sub>1 \<union> prog_rgs c\<^sub>2" |
+    "prog_rgs (While b I c) = priv (deps\<^sub>B b) \<union> prog_rgs c" |
+    "prog_rgs (DoWhile I c b) = priv (deps\<^sub>B b) \<union> prog_rgs c"
+
+fun prog_glbs
+  where 
+    "prog_glbs Skip = {}" |
+    "prog_glbs (Op v e f) = shr (rd e) \<union> shr (wr e)" |
+    "prog_glbs (Seq c\<^sub>1 c\<^sub>2) = prog_glbs c\<^sub>1 \<union> prog_glbs c\<^sub>2" |
+    "prog_glbs (If b c\<^sub>1 c\<^sub>2) = shr (deps\<^sub>B b) \<union> prog_glbs c\<^sub>1 \<union> prog_glbs c\<^sub>2" |
+    "prog_glbs (While b I c) = shr (deps\<^sub>B b) \<union> prog_glbs c" |
+    "prog_glbs (DoWhile I c b) = shr (deps\<^sub>B b) \<union> prog_glbs c"
+
+fun prog_ops
+  where 
+    "prog_ops Skip = {}" |
+    "prog_ops (Op v e f) = { (\<lfloor>v,e,f\<rfloor>) }" |
+    "prog_ops (Seq c\<^sub>1 c\<^sub>2) = prog_ops c\<^sub>1 \<union> prog_ops c\<^sub>2" |
+    "prog_ops (If b c\<^sub>1 c\<^sub>2) = { (\<lfloor>cmp b\<rfloor>) } \<union> prog_ops c\<^sub>1 \<union> prog_ops c\<^sub>2" |
+    "prog_ops (While b I c) = { (\<lfloor>cmp b\<rfloor>) } \<union> prog_ops c" |
+    "prog_ops (DoWhile I c b) = { (\<lfloor>cmp b\<rfloor>) } \<union> prog_ops c"
+*)
+
+fun glbs
+  where
+    "glbs p = rds p \<union> wrs p"
+
+definition all_points
+  where "all_points rs gs os \<equiv> {p. op p \<in> os \<and> rgs p \<subseteq> rs \<and> wrs p \<subseteq> gs \<and> rds p \<subseteq> gs}"
+
+lemma bound:
+  "upd2 R c P \<subseteq> all_points (com_rgs c \<union> \<Union> (rgs ` P)) (com_glbs c \<union> \<Union> (glbs ` P)) (basics c \<union> (op ` P))"
+  sorry
+
+lemma finite_all_points:
+  "finite rs \<Longrightarrow> finite gs \<Longrightarrow> finite os \<Longrightarrow> finite (all_points rs gs os)"
+  unfolding all_points_def sorry
+
+lemma upd_While:
+  fixes b c P R
+  assumes "finite P"
+  defines "f == (\<lambda>Y. (P \<union> upd2 R c Y))"
+  shows "upd2 R (Loop c) P = while (\<lambda>Y. f Y \<noteq> Y) f {}" (is "_ = ?r")
+proof -
+  let ?V = "all_points (com_rgs c \<union> \<Union> (rgs ` P)) (com_glbs c \<union> \<Union> (glbs ` P)) (basics c \<union> (op ` P))"
+  have "lfp f = ?r"
+  proof(rule lfp_while[where C = "?V"])
+    show "mono f" using f_def mono_union_upd2 by blast
+  next
+    fix Y show "Y \<subseteq> ?V \<Longrightarrow> f Y \<subseteq> ?V"
+      unfolding f_def using bound[of R c] by blast
+  next
+    show "finite ?V" using \<open>finite P\<close>
+      apply (intro finite_all_points)
+      by simp
+  qed
+  thus ?thesis by (simp add: f_def)
+qed
+
+lemma upd_While_let: "finite X \<Longrightarrow> upd2 R (Loop c) X =
+  (let f = (\<lambda>Y. X \<union> upd2 R c Y)
+   in while (\<lambda>Y. f Y \<noteq> Y) f {})"
+by(simp add: upd_While)
+
+lemma upd_While_set: "upd2 R (Loop c) (set xs) =
+  (let f = (\<lambda>Y. set xs \<union> upd2 R c Y)
+   in while (\<lambda>Y. f Y \<noteq> Y) f {})"
+by(rule upd_While_let, simp)
+
+lemmas [code] = upd2.simps(1,2,4,5) upd_While_set
+
+
+end
