SimAsm/SimAsm_WP.thy
@@ -1,0 +1,152 @@
+theory SimAsm_WP
+  imports SimAsm
+begin
+
+section \<open>Wellformedness\<close>
+
+definition glb
+  where "glb m \<equiv> \<lparr> st = (\<lambda>v. st m (Glb v)), \<dots> = more m \<rparr>"
+
+definition rg
+  where "rg m \<equiv> \<lambda>v. st m (Reg v)"
+
+definition stabilize
+  where "stabilize R P \<equiv> {m. \<forall>m'. (glb m,glb m') \<in> R \<longrightarrow> rg m = rg m' \<longrightarrow> m' \<in> P}"
+
+definition reflexive
+  where "reflexive R \<equiv> \<forall>m. (m,m) \<in> R"
+
+definition transitive
+  where "transitive R \<equiv> \<forall>m m' m''. (m,m') \<in> R \<longrightarrow> (m',m'') \<in> R \<longrightarrow> (m,m'') \<in> R"
+
+definition assert
+  where "assert b \<equiv> {m. b}"
+
+text \<open>Lift a relational predicate and assume it preserves the thread state\<close>
+definition step\<^sub>t :: "('v,'g,'a) grel \<Rightarrow> ('v,'g,'r,'a) trel"
+  where "step\<^sub>t R \<equiv> {(m,m'). (glb m, glb m') \<in> R \<and> rg m = rg m'}"
+
+text \<open>Lift a relational predicate\<close>
+definition step :: "('v,'g,'a) grel \<Rightarrow> ('v,'g,'r,'a) trel"
+  where "step R \<equiv> {(m,m'). (glb m, glb m') \<in> R}"
+
+text \<open>Define stability in terms of a relational predicate that preserves the thread state\<close>
+abbreviation stable\<^sub>t
+  where "stable\<^sub>t R P \<equiv> stable (step\<^sub>t R) P"
+
+text \<open>Couple all wellformedness conditions into a single definition\<close>
+abbreviation wellformed :: "('v,'g,'a) grel \<Rightarrow> ('v,'g,'a) grel \<Rightarrow> bool"
+  where "wellformed R G \<equiv> reflexive R \<and> transitive R \<and> reflexive G" 
+
+text \<open>Show that a stabilized predicate is stable\<close>
+lemma stabilize_stable [intro]:
+  assumes wf: "wellformed R G"
+  shows "stable\<^sub>t R (stabilize R Q)"
+  unfolding stable_def step\<^sub>t_def
+proof (clarsimp)
+  fix m m'
+  assume a: "m \<in> stabilize R Q" "(glb m, glb m') \<in> R" "rg m = rg m'"
+  have "\<forall>g''. (glb m',g'') \<in> R \<longrightarrow> (glb m,g'') \<in> R"
+    using assms a(2) unfolding transitive_def by blast
+  thus "m' \<in> stabilize R Q" using a(1,3) by (auto simp: stabilize_def)
+qed
+
+text \<open>The conjunction of two stable predicates is stable\<close>
+lemma stable\<^sub>t_conj [intro]:
+  assumes "stable\<^sub>t R P" "stable\<^sub>t R Q"
+  shows "stable\<^sub>t R (P \<inter> Q)"
+  using assms by (auto simp: stable_def)
+
+text \<open>Elimination rule to ignore the stabilization process\<close>
+lemma stabilizeE:
+  assumes "m \<in> stabilize R P"
+  assumes "reflexive R"
+  obtains "m \<in> P"
+proof -
+  have "\<forall>g. (glb m, glb g) \<in> R \<longrightarrow> rg m = rg g \<longrightarrow> g \<in> P" "(glb m, glb m) \<in>  R"
+    using assms by (auto simp: reflexive_def stabilize_def)
+  thus ?thesis using that by auto
+qed
+
+text \<open>Stabilization preserves entailment\<close>
+lemma stabilize_entail :
+  assumes "m \<in> stabilize R P" 
+  assumes "reflexive R"
+  assumes "P \<subseteq> Q"
+  shows "m \<in> stabilize R Q"
+  using assms by (auto simp: stabilize_def)
+
+section \<open>Predicate Transformations\<close>
+
+text \<open>Transform a predicate based on an sub-operation\<close>
+fun wp\<^sub>i :: "('v,'g,'r) op \<Rightarrow> ('v,'g,'r,'a) trans" 
+  where 
+    "wp\<^sub>i (assign r e) Q = {m. (m (r :=\<^sub>s ev m e)) \<in> Q}" |
+    "wp\<^sub>i (cmp b) Q =  {m. ev\<^sub>B m b \<longrightarrow> m \<in> Q}" | 
+    "wp\<^sub>i _ Q = Q"
+
+text \<open>Transform a predicate based on an auxiliary state update\<close>
+fun wp\<^sub>a :: "('v,'g,'r,'a) auxfn \<Rightarrow> ('v,'g,'r,'a) trans"
+  where "wp\<^sub>a a Q = {m. m(aux: a) \<in> Q}"
+
+text \<open>Transform a predicate based on a program c within an environment R\<close>
+fun wp :: "('v,'g,'a) grel \<Rightarrow> ('v,'g,'r,'a) lang \<Rightarrow> ('v,'g,'r,'a) trans"
+  where
+    "wp R Skip Q = Q" |
+    "wp R (Op v a f) Q = stabilize R (v \<inter> wp\<^sub>i a (wp\<^sub>a f Q))" |
+    "wp R (Seq c\<^sub>1 c\<^sub>2) Q = wp R c\<^sub>1 (wp R c\<^sub>2 Q)" |
+    "wp R (If b c\<^sub>1 c\<^sub>2) Q = stabilize R (wp\<^sub>i (cmp b) (wp R c\<^sub>1 Q) \<inter> wp\<^sub>i (ncmp b) (wp R c\<^sub>2 Q))" |
+    "wp R (While b I c) Q = 
+      (stabilize R I \<inter> assert (I \<subseteq> wp\<^sub>i (cmp b) (wp R c (stabilize R I)) \<inter> wp\<^sub>i (ncmp b) Q))" |
+    "wp R (DoWhile I c b) Q = 
+      (stabilize R I \<inter> assert (I \<subseteq> wp R c (stabilize R (wp\<^sub>i (cmp b) (stabilize R I) \<inter> wp\<^sub>i (ncmp b) Q))))"
+
+text \<open>Convert a predicate transformer into a relational predicate transformer\<close>
+definition wp\<^sub>r :: "('v,'g,'r,'a) trans \<Rightarrow> ('v,'g,'r,'a) rtrans"
+  where "wp\<^sub>r f G \<equiv> {(m,m'). m' \<in> f {m'. (m,m') \<in> G}}"
+
+subsection \<open>Guarantee Checks\<close>
+
+text \<open>Convert a predicate transformer into a guarantee check\<close>
+abbreviation guar
+  where "guar f G \<equiv> {m. (m,m) \<in> (wp\<^sub>r f G)}"
+
+text \<open>Ensure all global operations in a thread conform to its guarantee\<close>
+fun guar\<^sub>c
+  where 
+    "guar\<^sub>c Skip G = True" |
+    "guar\<^sub>c (Op v a f) G = (v \<subseteq> guar (wp\<^sub>i a o wp\<^sub>a f) (step G))" |
+    "guar\<^sub>c (Seq c\<^sub>1 c\<^sub>2) G = (guar\<^sub>c c\<^sub>1 G \<and> guar\<^sub>c c\<^sub>2 G)" |
+    "guar\<^sub>c (If _ c\<^sub>1 c\<^sub>2) G = (guar\<^sub>c c\<^sub>1 G \<and> guar\<^sub>c c\<^sub>2 G)" |
+    "guar\<^sub>c (While _ _ c) G = (guar\<^sub>c c G)" |
+    "guar\<^sub>c (DoWhile _ c _) G = (guar\<^sub>c c G)"
+
+section \<open>Locale Interpretation\<close>
+
+text \<open>Convert the language into the abstract language expected by the underlying logic\<close> 
+fun lift\<^sub>c :: "('v,'g,'r,'a) lang \<Rightarrow> (('v,'g,'r,'a) auxop, ('v,'g,'r,'a) state) com"
+  where
+    "lift\<^sub>c Skip = com.Nil" |
+    "lift\<^sub>c (Op v a f) = Basic (\<lfloor>v,a,f\<rfloor>)" |
+    "lift\<^sub>c (lang.Seq c\<^sub>1 c\<^sub>2) = (com.Seq (lift\<^sub>c c\<^sub>1) (lift\<^sub>c c\<^sub>2))" |
+    "lift\<^sub>c (If b c\<^sub>1 c\<^sub>2) = (Choice 
+      (com.Seq (Basic (\<lfloor>cmp b\<rfloor>)) (lift\<^sub>c c\<^sub>1)) (com.Seq (Basic (\<lfloor>ncmp b\<rfloor>)) (lift\<^sub>c c\<^sub>2)))" |
+    "lift\<^sub>c (While b I c) = (com.Seq ((com.Seq (Basic (\<lfloor>cmp b\<rfloor>)) (lift\<^sub>c c))*) (Basic (\<lfloor>ncmp b\<rfloor>)))" | 
+    "lift\<^sub>c (DoWhile I c b) = (lift\<^sub>c c ;; Basic (\<lfloor>cmp b\<rfloor>))* ;; lift\<^sub>c c ;; Basic (\<lfloor>ncmp b\<rfloor>)" 
+
+text \<open>The language is always thread-local\<close>
+lemma local_lift [intro]:
+  "local (lift\<^sub>c c)"
+  by (induct c) auto
+
+text \<open>Correctness of the guarantee check\<close>
+lemma com_guar:
+  "wellformed R G \<Longrightarrow> guar\<^sub>c c G \<Longrightarrow> \<forall>\<beta>\<in>basics (lift\<^sub>c c). guar\<^sub>\<alpha> \<beta> (step G)"
+proof (induct c) 
+  case (Op v p)
+  then show ?case by (cases p) (auto simp: liftg_def guar_def wp\<^sub>r_def)
+qed (auto simp: guar_def reflexive_def liftl_def step_def)
+
+interpretation rules fwd\<^sub>s re\<^sub>a by (unfold_locales) (auto)
+
+end
